proof/amd64/avx2/Keccakf1600_avx2.ec
@@ -67,14 +67,14 @@ qed.
 lemma keccakf1600_pround_avx2_ll: islossless M.__keccakf1600_pround_avx2 
 by islossless.
 
-pragma +Circuit:timing.
+(*pragma +Circuit:timing.*)
 
 hoare keccak_pround_avx2_h _a:
  M.__keccakf1600_pround_avx2 :
  state = _a /\ stavx2INV _a ==> res = stavx2_keccak_pround _a.
 proof.
 proc.
-circuit.
+by circuit.
 qed.
 
 lemma keccakf1600_avx2_ll': islossless M.__keccakf1600_avx2.
